Fix WP of EStoreId

theories/rules/rules_EStoreId.v
@@ -18,14 +18,17 @@ Section cap_lang_rules.
   Implicit Types mem : Mem.
   Implicit Types lmem : LMem.
 
-  Inductive EStoreId_spec (lregs lregs' : LReg) (lmem lmem' : LMem) (rs rd : RegName) (any : LWord) otype tidx : cap_lang.val -> Prop :=
+  Inductive EStoreId_spec (lregs lregs' : LReg) (rs rd : RegName) (any : LWord) otype tidx : cap_lang.val -> Prop :=
   | EStoreId_spec_success:
+    incrementLPC (<[ rs := (LWInt otype) ]> (<[rd := any]> lregs)) = Some lregs' →
     has_seal otype tidx → (* we associate a given table index with the provided otype *)
-    lregs !! rs = Some (LWInt otype) →
-    lregs !! rd = Some any →
-    EStoreId_spec lregs lregs' lmem lmem' rs rd any otype tidx NextIV
-  |EStoreId_spec_failure:
-    EStoreId_spec lregs lregs' lmem lmem' rs rd any otype tidx FailedV.
+    EStoreId_spec lregs lregs' rs rd any otype tidx NextIV
+  |EStoreId_spec_failure_incr_pc:
+    incrementLPC lregs = None →
+    lregs = lregs' →
+    EStoreId_spec lregs lregs' rs rd any otype tidx FailedV.
+  (* |EStoreId_spec_failure_other: *)
+  (*   EStoreId_spec lregs lregs' rs rd any otype tidx FailedV. *)
 
   (* TODO @Denis *)
   (* The EStoreId instruction fetches the machine's stored hash for a given OType.
@@ -35,53 +38,50 @@ Section cap_lang_rules.
   (* Essentially it gives us a partial view on the enclave table, since we now know that at a particular index, at some point, there was an enclave with a particular identity. *)
   (* In a later step of the verification, an invariant will allow us to trade this resource for the specific predicate that always holds for results signed by enclaves with that hash... *)
   (* This enables "learning" some information about the signed, yet unknown result: we will be able to establish that at least the above predicate will hold for it... *)
-  Lemma wp_estoreid E pc_p pc_b pc_e pc_a pc_a' pc_v lw rd rs otype any lregs lmem :
+  Lemma wp_estoreid E pc_p pc_b pc_e pc_a pc_v lw rd rs otype any lregs :
     decodeInstrWL lw = EStoreId rd rs →
     isCorrectLPC (LCap pc_p pc_b pc_e pc_a pc_v) →
-    (pc_a + 1)%a = Some pc_a' →
-    regs_of (EStoreId rs rd) ⊆ dom lregs →
+    regs_of (EStoreId rd rs) ⊆ dom lregs →
     lregs !! PC = Some (LCap pc_p pc_b pc_e pc_a pc_v) →
 
     {{{ (▷ [∗ map] k↦y ∈ lregs, k ↦ᵣ y) ∗
         (pc_a, pc_v) ↦ₐ lw }}}
       Instr Executable @ E
-    {{{ lregs' lmem' tidx retv, RET retv;
-        ⌜ EStoreId_spec lregs lregs' lmem lmem' rs rd any otype tidx retv⌝ ∗
+    {{{ lregs' tidx retv, RET retv;
+        ⌜ EStoreId_spec lregs lregs' rs rd any otype tidx retv⌝ ∗
         ([∗ map] k↦y ∈ lregs', k ↦ᵣ y) ∗
         (pc_a, pc_v) ↦ₐ lw ∗
         rs ↦ᵣ LWInt otype ∗
         if decide (retv = NextIV) then
-          PC ↦ᵣ LCap pc_p pc_b pc_e pc_a' pc_v ∗
           ∃ (I : EIdentity),
             rd ↦ᵣ (LWInt I) ∗
             enclave_all tidx I (*!*)
         else
-          PC ↦ᵣ LCap pc_p pc_b pc_e pc_a pc_v ∗
           rd ↦ᵣ any }}}.
   Proof.
-    iIntros (Hinstr Hvpc Dregs HPC HPCa φ) "(>Hrmap & Hpca) Hφ".
+    iIntros (Hinstr Hvpc Dregs HPC φ) "(>Hrmap & Hpca) Hφ".
+    iApply (wp_instr_exec_opt Hvpc HPC Hinstr Dregs with "[$Hpca $Hrmap Hφ]").
+    iModIntro.
+    iIntros (σ1) "(Hσ1 & Hmap &Hpc_a)".
+    iModIntro.
+    iIntros (wa) "(%Hrpc & %Hmema & %Hcorrpc & %Hdecode) Hcred".
     apply isCorrectLPC_isCorrectPC_iff in Hvpc; cbn in Hvpc.
-    iApply wp_lift_atomic_head_step_no_fork; auto.
-    iIntros (σ1 ns l1 l2 nt) "Hσ1 /=".
-    iDestruct "Hσ1" as (lr lm vmap) "(% & % & % & Hr & Hm & %Hcur & Henc_cur & Henc_prev & Henc_all & HEC & %Hdisj & %Hdom & %Hdisj2 & %Union_all & %State)".
-    all: admit.
-    (* iDestruct (@gen_heap_valid with "Hr Hpc") as %?. *)
-    (* iDestruct (@gen_heap_valid with "Hm Hpca") as %?. *)
-    (* iModIntro. *)
-    (* iSplitR. by iPureIntro; apply normal_always_head_reducible. *)
-    (* iIntros (e2 σ2 efs Hstep). *)
-    (* apply prim_step_exec_inv in Hstep as (-> & -> & (c & -> & Hstep)). *)
-    (* iNext; iIntros "_". *)
-    (* iSplitR; auto. *)
-    (* iModIntro. *)
-    (* rewrite -/((lword_get_word (LCap pc_p pc_b pc_e pc_a pc_v))). *)
-    (* 2: eapply state_corresponds_mem_correct_PC ; eauto; cbn ; eauto. *)
-    (* cbn in Hstep; simplify_eq. *)
-    (* iModIntro. *)
-    (* iSplitR "Hφ Hpc Hpca". last (iApply "Hφ" ; iFrame). *)
-   (*  iExists lr, lm, vmap. *)
-   (*  iFrame; auto. *)
-   (* Qed. *)
+
+    iApply wp_wp2.
+
+    iMod (state_interp_transient_intro (lm:= ∅) with "[$Hmap $Hσ1]") as "Hσ".
+    { by rewrite big_sepM_empty. }
+
+    iApply wp_opt2_bind.
+    iApply wp_opt2_eqn_both.
+    iApply (wp2_reg_lookup with "[$Hσ Hφ Hcred Hpc_a]") ; first by set_solver.
+    iIntros (lwrs) "Hσ %HrsL %Hrs".
+
+    iApply wp_opt2_bind.
+    assert ((get_otype_from_wint (lword_get_word lwrs) = finz.of_z otype)). admit.
+    rewrite H.
+    iApply wp_opt2_eqn_both.
+
   Admitted.
 
   Lemma wp_estoreid_success_unknown E pc_p pc_b pc_e pc_a pc_a' pc_v lw rd rs otype any :
@@ -112,16 +112,31 @@ Section cap_lang_rules.
     iIntros (Hinstr Hvpc Hpca φ) "(>HPC & >Hpc_a & >Hrs & >Hrd) Hφ".
     iDestruct (map_of_regs_3 with "HPC Hrs Hrd") as "[Hrmap (%&%&%)]".
 
+    (* iDestruct (big_opM_delete with "H"). *)
     iApply (wp_estoreid with "[$Hrmap $Hpc_a]"); eauto; simplify_map_eq; eauto.
     { by unfold regs_of; rewrite !dom_insert; set_solver+. }
-    Unshelve. 4: apply gmap_empty. (* empty LMem ? *)
 
-    iNext. iIntros (lregs' lmem' tidx retv) "(#Hspec & Hrmap & HPCa & Hrs & Hpost)".
+
+    iNext. iIntros (lregs' tidx retv) "(#Hspec & Hrmap & HPCa & Hrs & Hpost)".
     iDestruct "Hspec" as %Hspec.
     destruct Hspec eqn:?; cycle 1; cbn; iApply "Hφ". iFrame.
     - iRight. auto.
-    - iFrame. iLeft. iDestruct "Hpost" as "(HPC & Henc)". iFrame. iSplitR. by iPureIntro.
-      iDestruct "Henc" as (I) "(Hrd & Henc)".
+      iDestruct "Hpost" as "Hrd". iFrame. iSplit. by iPureIntro. subst.
+      rewrite big_opM_insert_delete. iDestruct "Hrmap" as "[$ Hrmap]".
+    - iFrame. iLeft. iDestruct "Hpost" as "[%I (Hrd & Henc)]". iFrame. iSplitR. by iPureIntro.
+      clear Heqe. apply incrementLPC_Some_inv in e as (?&?&?&?&?&?&?&?&?).
+      subst.
+
+      rewrite big_opM_insert_delete.
+
+      rewrite lookup_insert_ne in H2; auto.
+      rewrite lookup_insert_ne in H2; auto.
+      rewrite lookup_insert in H2.
+      inversion H2; subst.
+
+      rewrite Hpca in H3. inversion H3; subst.
+
+       iDestruct "Hrmap" as "[$ Hrmap]".
       iExists I, tidx. iFrame. by iPureIntro.
   Qed.
 
